\chapter{Useful Laplace Transforms}
\label{chapter:usefullaplacetransforms}

\section{Table of Transforms}

\begin{table}[h]
\begin{center}
\begin{tabular}{c c}
\hline\hline
$f(t) = \mathcal{L}^{-1}\left\{ F(s) \right\}$   &   $F(s) = \mathcal{L}\left\{ f(t) \right\} $ \\
\hline\hline
$f(t)$                                       & $F(s)$                  \\
$f'(t)$                                      & $sF(s) - f(0)$          \\
$a$                                          & $\frac{a}{s}$           \\
$\exp(-at)$                                   & $\frac{1}{s+a}$         \\
$a \exp(-bt)$                                 & $\frac{a}{s+b}$         \\
$\frac{1}{a} \left[1 - \exp(-at)\right]$      & $\frac{a}{s(s+a)}$      \\
$\frac{a}{b} \left[1 - \exp(-bt)\right]$      & $\frac{a}{s(s+b)}$      \\
\hline\hline
\end{tabular}
\end{center}
\caption{Useful Laplace transforms}
\label{table:usefullaplacetranforms}
\end{table}


\section{Decay with a Source Term}

Set up the equation:

\begin{equation}
\begin{split}
\frac{dN(t)}{dt} = \omega - \lambda N(t)
\end{split}
\label{eq:decaysourceterm1}
\end{equation}

Transform:

\begin{equation}
\begin{split}
\mathcal{L}\left\{  \frac{dN(t)}{dt}       \right\} = sF(s) - N_{0} \\
\mathcal{L}\left\{  \omega - \lambda N(t)  \right\} = \frac{\omega}{s} - \lambda N(s) \\
\end{split}
\label{eq:decaysourceterm2}
\end{equation}
 
Rearrange to make $N(s)$ the subject:

\begin{equation}
\begin{split}
sN(s) - N_{0} = \frac{\omega}{s} - \lambda N(s) \\
(s + \lambda) N(s) = \frac{\omega}{s} + N_{0} \\
N(s) = \frac{\omega}{s(s + \lambda)} + \frac{N_{0}}{(s + \lambda)} \\
\end{split}
\label{eq:decaysourceterm3}
\end{equation}

Inverse transform:

\begin{equation}
\begin{split}
\mathcal{L}^{-1}\left\{  N(s)    \right\} = N(t) \\
\mathcal{L}^{-1}\left\{  \frac{\omega}{s(s + \lambda)}   \right\} = \frac{\omega}{\lambda} \left(1 - \exp(-\lambda t)\right) \\
\mathcal{L}^{-1}\left\{  \frac{N_{0}}{s + \lambda}   \right\} = N_{0} \exp(-\lambda t) \\
\end{split}
\label{eq:decaysourceterm3}
\end{equation}

Simplify:

\begin{equation}
\begin{split}
N(t) = \frac{\omega}{\lambda} \left(1 - \exp(-\lambda t)\right) + N_{0} \exp(-\lambda t)\\
N(t) = \frac{\omega}{\lambda} + \left(N_{0} - \frac{\omega}{\lambda} \right) \exp(-\lambda t) \\
\end{split}
\label{eq:decaysourceterm3}
\end{equation}









