\newcommand{\eqForceMatchingA}{
\begin{equation}
\begin{split}
Z(\vec{\alpha}) = Z_F(\vec{\alpha}) + Z_C(\vec{\alpha})
\end{split}
\label{eq:eqForceMatchingA}
\end{equation}
}

\newcommand{\eqForceMatchingB}{
\begin{equation}
\begin{split}
Z_F(\vec{\alpha}) = \frac{1}{ 3 \sum _{k=1}^M N_k} \sum _{k=1}^M \sum _{i=1} ^{N_k} \lvert \vec{F}_{ki} (\vec{\alpha}) - \vec{F ^0_{ki}} \rvert^2
\end{split}
\label{eq:eqForceMatchingB}
\end{equation}
}

\newcommand{\eqForceMatchingC}{
\begin{equation}
\begin{split}
Z_C(\vec{\alpha}) = \sum _{r=1}^{N_C} W_r \left[ \right]
\end{split}
\label{eq:eqForceMatchingC}
\end{equation}
}
